theories/TM/Code/Decode.v
@@ -1,0 +1,24 @@
+From Undecidability.TM Require Import TM.
+
+Module ContainsEncoding.
+  Section containsEncoding.
+    Local Unset Implicit Arguments.
+
+    Context {sig:Type} {n:nat} {X:Type}.
+    Context (encode : X -> list sig).
+    (*Hypothesis (nonEmpty : forall x, encode x <> []).*)
+
+    Definition Rel : pRel sig bool 1 :=
+      fun tin '(yout, tout) =>
+        match yout with
+          true => exists (x:X) t__L t__R,
+                 let t__x := encode x in
+                 (exists c__hd, hd_error t__x = Some c__hd /\  tin[@Fin0] = midtape t__L c__hd (tl t__x++t__R) )
+                 /\ exists c__last, hd_error (rev t__x) = Some c__last /\ tout[@Fin0] = midtape (tl(rev t__x)++ t__L) c__last t__R
+        | false => forall t__L (x:X) t__R,
+            let t__x := encode x in
+            exists c__hd, hd_error t__x = Some c__hd /\
+            tin[@Fin0] <> midtape t__L c__hd (tl t__x++t__R)
+        end.
+  End containsEncoding.
+End ContainsEncoding.
