theories/TM/Single/DecodeTapes.v
@@ -1,0 +1,362 @@
+From Undecidability.TM Require Import TM ProgrammingTools Code.Decode.
+
+From Undecidability.TM Require Single.EncodeTapes Single.StepTM Single.EncodeTapesInvariants CaseList.
+Require Import FunInd Lia Ring Arith.
+
+From Coq.ssr Require Import ssrfun.
+Module CheckEncodesTape.
+  Section checkEncodesTape.
+
+    Import EncodeTapes StateWhile CaseList Mono Multi MoveToSymbol Copy Switch If Combinators Single.EncodeTapesInvariants.
+    
+    Context (sig:finType) (n:nat).
+    
+    Notation sig__M := (FinType(EqType(sigTape sig))).
+
+    Definition Rel : pRel sig__M bool 1 := ContainsEncoding.Rel (encode_tape (sig:=sig)).
+
+    Definition M2 x :pTM sig__M bool 1 := if negb (Option.apply (@isMarked sig) false x)
+                                 then Return Nop false
+                                 else
+                                   MoveToSymbol (fun x => isMarked x || isLeftBlank x || isRightBlank x || isNilBlank x) id;;
+                                   Relabel ReadChar (Option.apply isRightBlank false).
+
+    Definition f__M2 x t : (bool*tape sig__M) :=
+      if negb (Option.apply (@isMarked sig) false x)
+      then (false,t)
+      else let t' := MoveToSymbol_Fun (fun x => isMarked x || isLeftBlank x || isRightBlank x) id t in
+           (Option.apply isRightBlank false (current t'),t').
+
+    Definition caseFirstSymbol : pTM sig__M (bool+bool) 1:=
+      Switch
+        ReadChar
+        (fun x =>
+           match x with
+             Some NilBlank => Return Nop (inl true)
+           | Some (LeftBlank b) => Return Nop (inr b)
+           | _ => Return Nop (inl false)
+           end).
+
+    Definition f__caseFirstSymbol (t: tape sig__M): (bool+bool):=
+      match current t with
+        Some NilBlank => inl true
+      | Some (LeftBlank b) => inr b
+      | _ => inl false
+      end.
+
+    Definition M__step : bool*bool -> pTM sig__M ((bool*bool) + bool) 1 :=
+      fun '(haveSeenMark,haveSeenSymbol) =>
+        Switch
+          ReadChar
+          (fun x =>
+             match x with
+               None => Return Nop (inr false)
+             | Some c =>
+               if (isMarked c && haveSeenMark) || isNilBlank c || isLeftBlank c || isRightBlank c
+               then Return Nop (inr (isRightBlank c && (xorb haveSeenMark (isMarked c)) && haveSeenSymbol))
+               else Return (Move R) (inl (haveSeenMark || isMarked c,haveSeenSymbol || isSymbol c))
+             end).
+
+    Definition f__step bs t : (bool * bool + bool) * tape sig__M :=
+      let (haveSeenMark,haveSeenSymbol) := (fst bs,snd bs) in
+      match current t with
+        None => (inr false,t)
+      | Some c =>
+        if (isMarked c && haveSeenMark) || isNilBlank c || isLeftBlank c || isRightBlank c
+        then (inr (isRightBlank c && (xorb haveSeenMark (isMarked c)) && haveSeenSymbol),t)
+        else (inl (haveSeenMark || isMarked c,haveSeenSymbol || isSymbol c),tape_move_right t)
+      end.
+
+    Definition M' (bs : bool*bool) := 
+      StateWhile M__step bs.
+
+    Function f' bs t { measure rlength t } : (bool * tape sig__M)  :=
+      let r := f__step bs t in
+      match fst r with 
+        inl bs' => f' bs' (snd r)
+      | inr b => (b,(snd r))
+      end.
+    Proof.
+      unfold f__step. intros [haveSeenMark haveSeenSymbol] [ | | | ? c t__R] ?;cbn.
+      1-3:now intros [=].
+      destruct c as [ [] | [] | | | ];cbn. all:try solve [inversion 1].
+      1-4:destruct haveSeenMark;cbn.
+      all:intros [= <-]. all:destruct t__R;cbn. all:nia.
+    Qed.
+    
+    Definition M : pTM sig__M bool 1:=
+      If (Relabel ReadChar (Option.apply isLeftBlank false))
+         (Switch ReadChar (fun c => Move R;; M' (Option.apply (@isMarked _) false c,false)))
+         (Relabel ReadChar (Option.apply isNilBlank false)).
+
+    Definition f (t : tape sig__M) : (bool*tape sig__M) :=
+      match current t with
+        None => (false,t)
+      | Some c =>
+        if isLeftBlank c then  f' (isMarked c,false) (tape_move_right t)
+        else (isNilBlank c, t)
+      end.
+
+    (** Verification*)
+
+
+    Local Arguments Vector.to_list {A n} (!v).
+
+    Local Arguments plus : simpl never.
+    Local Arguments mult : simpl never.
+    Local Arguments caseFirstSymbol : simpl never.
+
+    Tactic Notation "destruct" "_" "in" constr(H):=
+      match type of H with
+      | context[match ?X with _ => _ end] => destruct X
+      | context[match ?X with _ => _ end] => destruct X
+      end.
+
+    Tactic Notation "tacInEvar" constr(E) tactic3(tac) :=
+      is_evar E;
+      let t := type of E in
+      let __tmp_callInEvar := fresh "__tmp_callInEvar" in
+      evar (__tmp_callInEvar:t);
+      (only [__tmp_callInEvar]:tac);unify E __tmp_callInEvar;subst __tmp_callInEvar;instantiate.
+
+    Tactic Notation "introsSwitch" ne_simple_intropattern_list(P):=
+      match goal with
+        |- (forall f' , ?REL _ (?R f')) =>
+        tacInEvar R intros P;cbn beta;intros P
+      end.
+
+
+
+    Tactic Notation "destructBoth" constr(g) "as" simple_intropattern(P) :=
+      match goal with
+        |- (?REL _ ?R) =>
+        tacInEvar R (destruct g as P);destruct g as P;cbn zeta iota
+      end.
+
+    
+    Tactic Notation "destructBoth" constr(g) :=
+      destructBoth g as [].
+
+    Lemma Realises__step bs : M__step bs ⊨ (fun t '(y,t')=> f__step bs t[@Fin0] = (y,t'[@Fin0])).
+    Proof.
+      destruct bs as (seenMark, seenSymbol). eapply Realise_monotone.
+      { unfold M__step;cbn. apply Switch_Realise. now TM_Correct.
+        introsSwitch c. destructBoth c as [c | ]. 2:now TM_Correct.
+        destructBoth (isMarked c && seenMark || isNilBlank c || isLeftBlank c || isRightBlank c). all:TM_Correct.
+      }
+      hnf;cbn. intros t (y&t') (?&?&[-> -> ]&H);revert H.
+      destruct current. 2:{ cbn. now intros (->&_&->). }
+      destruct _. all:cbn. all:intros (->&_&->). all:easy.
+    Qed.
+
+    Tactic Notation "infTer" int_or_var(n) :=
+      let t := try (first [simple eapply ex_intro | simple apply conj | simple eapply Nat.le_refl])
+      in t;do n t.
+    
+    Lemma Terminates__step bs : projT1 (M__step bs) ↓ (fun _ k => 3 <= k).
+    Proof.
+      destruct bs as (seenMark, seenSymbol). eapply TerminatesIn_monotone.
+      { unfold M__step;cbn. apply Switch_TerminatesIn. 1,2:now TM_Correct.
+        introsSwitch c. destructBoth c as [c | ]. 2:now TM_Correct.
+        destructBoth (isMarked c && seenMark || isNilBlank c || isLeftBlank c || isRightBlank c). all:TM_Correct.
+      }
+      hnf;cbn. intros t y Hy. infTer 3. rewrite <- Hy.
+      2:{ intros ? ? [-> ->]. destruct current. 2:lia. destruct _. 2:reflexivity. nia. }
+      nia.
+    Qed.
+    
+    Lemma Realises : M ⊨ (fun tin '(b,tout) => f tin[@Fin0] = (b,tout[@Fin0])).
+    Proof.
+      eapply Realise_monotone.
+      { unfold M. TM_Correct_step. 1,3:now TM_Correct.
+        apply Switch_Realise. now TM_Correct.
+        cbn;intros c. TM_Correct_step. now TM_Correct.
+        unfold M'.
+        eapply Realise_monotone with
+            (R:= fun t '(y,t')=> f' (oapp (isMarked (sig:=eqType_X (type sig))) false c, false) t[@Fin0] = (y,t'[@Fin0])).
+        { eapply StateWhile_Realise. now eapply Realises__step. }
+        generalize (oapp (isMarked (sig:=eqType_X (type sig))) false c, false) as bs. clear c.
+        apply StateWhileInduction. all:cbn - [f__step].
+        -intros t bs b' t'. rewrite f'_equation. intros ->. reflexivity. 
+        -intros t bs bs' t' t'' v'. rewrite f'_equation with (t:=t[@Fin0]). intros -> <-. reflexivity.
+      }
+      hnf;cbn.
+      intros t (y&t1) [H |H];revert H.
+      all:intros (?&(?&H1&->&->)&H);revert H.
+      -intros (?&?&[-> ->]&_&t2&Ht2&<-).
+       unfold f. destruct current. 2:now inv H1.
+       cbn in H1. rewrite <- H1. cbn. congruence.
+      -intros (?&->&->&->). unfold f.
+       destruct current. 2:easy.
+       cbn in *. now rewrite <- H1. 
+    Qed.
+
+    
+    Definition Ter : tRel sig__M 1:=
+      fun t k => 4 * (| tape_local (tape_move_right t[@Fin0]) |) + 9 <= k.
+
+    Lemma Terminates : projT1 M ↓ Ter.
+    Proof.
+      eapply TerminatesIn_monotone.
+      { unfold M. TM_Correct_step. 1,2,4:TM_Correct.
+        apply Switch_TerminatesIn. 1,2:TM_Correct.
+        cbn;intros c. TM_Correct_step. 1,2:now TM_Correct.
+        unfold M'.
+        eapply TerminatesIn_monotone. 1:{ TM_Correct_step. now eapply Realises__step. now apply Terminates__step. }
+        evar (c0:nat).
+        evar (time : nat -> nat). [time]:intros n0.
+        apply StateWhileCoInduction with (T:= fun _ t k => time (length (tape_local t[@Fin0])) +c0 <= k). all:cbn - [f__step].
+        -intros l t k Hk. infTer 2. intros y' t'.
+         unfold f__step. destruct current eqn:Hc.
+         2:{intros [= <- _]; rewrite <- Hk. enough (3 <= c0). now nia. shelve. }
+         destruct _ eqn:Hs. all: intros [= <- Ht']. 1:{ enough (3 <= c0). now nia. shelve. }
+         rewrite <- Ht'. infTer 2. rewrite <- Hk.
+         destruct t[@Fin0] as [ | | | ? ? t__R]. 1-3:easy. destruct t__R;cbn.
+         [time]:refine (n0*4). all:unfold time. all: nia.
+      } Unshelve. [c0]:exact 3. 2-3:subst c0;nia.
+      cbn. intros ? ? HT. infTer 5.
+      2:{ intros t ? (?&->&->&<-). destruct _.
+          { infTer 5. intros ? ? [-> ->]. infTer 5. intros ? ? ->. reflexivity. }
+          nia.
+      }
+      ring_simplify. hnf in HT. cbn in *. nia.
+    Qed.
+    
+    Lemma f'_spec (seenMark seenSymbol : bool) t__L' b t__L c t__R res:
+      (length (filter (@isMarked _) (t__L'++[LeftBlank b])) = if seenMark then 1 else 0)
+      -> (forall x, x el t__L' -> isSymbol x = true)
+      -> reflect (t__L' <> []) seenSymbol
+      -> res =  f' (seenMark,seenSymbol) (midtape (t__L'++LeftBlank b::t__L) c t__R)
+      ->  if fst res then
+           exists (x:tape sig) (t__R1 t__R2 : list sig__M),
+             t__R = t__R1++t__R2
+             /\ encode_tape x = LeftBlank b :: rev t__L'++c::t__R1
+             /\ snd res = midtape (tail (rev t__R1++[c])++t__L'++LeftBlank b::t__L) (hd c (rev t__R1++[c])) t__R2
+         else
+           forall x (t__R1 t__R2 : list sig__M),
+             t__R = t__R1++t__R2 -> 
+             encode_tape x <> LeftBlank b :: rev t__L'++c::t__R1.
+    Proof.
+      remember (length t__R) as n0 eqn: Hn0. revert t__R Hn0 t__L' c res seenMark seenSymbol.
+      induction n0 as [n0 IH] using lt_wf_ind. intros ? -> ? ? res ? ?;cbn in *.
+      intros H__seenMark H__symbs H__seenSymbol Hres. 
+      rewrite f'_equation in Hres.
+      destruct c;cbn. 1-3:clear IH.
+      -replace (res.1) with false.
+       2:{ cbn in Hres. destruct marked;cbn in Hres. destruct seenMark in Hres;cbn in Hres. all:now subst. }
+       clear - H__symbs.
+       intros ? ? ? -> (Hneq&Hsym&(?&Hlast)&_)%encode_tape_invariants_partial;cbn in *. 2:now setoid_rewrite <- in_rev.
+       destruct t__R1. easy. discriminate (Hsym (LeftBlank marked)). rewrite tl_app. 2:now length_not_eq. now eauto.     
+      -revert Hres. cbn. rewrite !orb_true_r.
+       destruct marked;cbn in *. destruct seenMark;cbn in *. all:intros ->;cbn. 3:destruct seenMark;cbn. 2,3:destruct seenSymbol;cbn.
+       +intros ? ? ? -> (Hneq&Hsym&(?&Hlast)&Hmarks)%encode_tape_invariants_partial;cbn in *. 2:now setoid_rewrite <- in_rev.
+        autorewrite with list in *. nia.
+       +edestruct invert_symbols_0_marked with (t:= t__L') as (t__R2&->).
+        1,2:autorewrite with list in *. now nia. now intros;eapply H__symbs.
+        destruct b. 1:{exfalso. autorewrite with list in H__seenMark. now cbn in H__seenMark;nia. } 
+        destruct t__R2 as [ | c' cs] eqn:Htp. 1:{exfalso. inversion H__seenSymbol. easy. } 
+        eexists (rightof _ _),[],_. repeat eapply conj. 1,3:reflexivity. cbn.
+        autorewrite with list;cbn.  setoid_rewrite <- map_rev with (l:=cs) at 2. easy.
+       +intros ? ? ? -> (Hneq&Hsym&(?&Hlast)&Hmarks&Hnempty)%encode_tape_invariants_partial;cbn in *. 2:now setoid_rewrite <- in_rev.
+        destruct t__L'. all:inv H__seenSymbol. 2:now apply H. cbn in *;autorewrite with list in *.
+        destruct t__R1. 2:{ ediscriminate (Hsym (RightBlank _)). rewrite tl_app. eauto. length_not_eq. }
+        cbn in *. nia.
+       +destruct b.
+        *edestruct invert_symbols_0_marked with (t:= t__L') as (t__R2&->).
+         1,2:autorewrite with list in *;cbn in *. now nia. now intros;eapply H__symbs.
+         destruct t__R2 eqn:?. 1:{exfalso. inversion H__seenSymbol. easy. }
+         destruct (rev t__R2) eqn:Htp. 1:{exfalso. subst. revert Htp. length_not_eq. } 
+         eexists (leftof _ _),[],_. repeat eapply conj. 1,3:reflexivity. rewrite <- Heql. cbn.
+         autorewrite with list;cbn.  setoid_rewrite <- map_rev with (l:=t__R2). now rewrite Htp.
+        *edestruct @invert_symbols_1_marked with (t:= t__L') as (?&?&?&->).
+         1,2:autorewrite with list in *;cbn in *. now nia. now intros;eapply H__symbs.
+         eexists (midtape _ _ _),[],_. repeat eapply conj. 1,3:reflexivity. cbn.
+         repeat (autorewrite with list;cbn).  setoid_rewrite map_rev. easy.
+       +intros ? ? ? -> (Hneq&Hsym&(?&Hlast)&Hmarks&?)%encode_tape_invariants_partial;cbn in *. 2:now setoid_rewrite <- in_rev.
+        destruct t__R1. 2:{ ediscriminate (Hsym (RightBlank _)). rewrite tl_app. 2:now length_not_eq. eauto. }
+        destruct t__L'. 2:{ inversion H__seenSymbol. now apply H0. }
+        cbn in *. nia.
+       +intros ? ? ? -> (Hneq&Hsym&(?&Hlast)&Hmarks&?)%encode_tape_invariants_partial;cbn in *. 2:now setoid_rewrite <- in_rev.
+        destruct t__R1. 2:{ ediscriminate (Hsym (RightBlank _)). rewrite tl_app. 2:now length_not_eq. eauto. }
+        cbn in *. autorewrite with list in *. nia.
+      -replace (res.1) with false.
+       2:{ cbn in Hres. destruct seenMark in Hres;cbn in Hres. all:now subst. }
+       clear - H__symbs.
+       intros ? ? ? -> (Hneq&Hsym&(?&Hlast)&_)%encode_tape_invariants_partial;cbn in *. 2:now setoid_rewrite <- in_rev.
+       destruct t__R1. easy. discriminate (Hsym (NilBlank)). rewrite tl_app. 2:now length_not_eq. now eauto.   
+      -revert Hres. cbn. destruct seenMark;cbn.
+       {clear IH. intros ->;cbn.
+        intros ? ? ? -> (Hneq&Hsym&(?&Hlast)&?&?)%encode_tape_invariants_partial;cbn in *. 2:now setoid_rewrite <- in_rev.
+        cbn in *. autorewrite with list in *. nia.
+       }
+       destruct t__R.
+       { clear IH. cbn. rewrite f'_equation;cbn.  
+         intros ->;cbn.
+         intros ? ? ? Hnil (Hneq&Hsym&(?&Hlast)&?&?)%encode_tape_invariants_partial;cbn in *. 2:now setoid_rewrite <- in_rev.
+         destruct t__R1. 2:easy. destruct t__R2. 2:easy. easy.
+       }
+       cbn. intros H.
+       autorewrite with list in H__seenMark. destruct b;cbn in H__seenMark. now nia. 
+       specialize IH with (t__L' := MarkedSymbol s :: t__L');cbn in IH. pose (H' := H);eapply IH in H';clear IH.
+       3:reflexivity. 2:nia. 2:now autorewrite with list in *;nia. 2:now intros ? [<- | ];eauto.
+       2:now rewrite orb_true_r;constructor.
+       destruct res as [[] t'];cbn in *.
+       +destruct H' as (x&t__R1&t__R2&->&Hx&->).
+        eexists x,(s0::t__R1),t__R2.
+        repeat (cbn in Hx|-*;autorewrite with list in Hx|-* ). split. 2:split. 1,2:congruence.
+        destruct (rev t__R1);cbn;now autorewrite with list.
+       +intros x ? ? H__R Hx. specialize encode_tape_invariants_partial with (1:=Hx) as (Hneq&Hsym&(?&Hlast)&_);cbn in *. now setoid_rewrite <- in_rev.
+        destruct (rev t__R1) eqn:Heq. all:inv Hlast.
+        destruct t__R1. now inv Heq. inv H__R. eapply H'. reflexivity.  rewrite Hx;cbn;autorewrite with list;cbn. reflexivity.
+      -revert Hres. cbn.
+       destruct t__R.
+       { clear IH. cbn. rewrite f'_equation;cbn.  
+         intros ->;cbn.
+         intros ? ? ? Hnil (Hneq&Hsym&(?&Hlast)&?&?)%encode_tape_invariants_partial;cbn in *. 2:now setoid_rewrite <- in_rev.
+         destruct t__R1. 2:easy. destruct t__R2. 2:easy. easy.
+       }
+       cbn;intros H.
+       specialize IH with (t__L' := UnmarkedSymbol s :: t__L');cbn in IH. pose (H' := H);eapply IH in H';clear IH.
+       3:reflexivity. 2:lia. 3:now intros ? [<- | ];eauto. 3:now rewrite orb_true_r;constructor.
+       2:{ autorewrite with list in *. destruct seenMark;cbn in *;nia. }
+       destruct res as [[] t'];cbn in *.
+       +destruct H' as (x&t__R1&t__R2&->&Hx&->).
+        eexists x,(s0::t__R1),t__R2.
+        repeat (cbn in Hx|-*;autorewrite with list in Hx|-* ). split. 2:split. 1,2:congruence.
+        destruct (rev t__R1);cbn;now autorewrite with list.
+       +intros x ? ? H__R Hx. specialize encode_tape_invariants_partial with (1:=Hx) as (Hneq&Hsym&(?&Hlast)&_);cbn in *. now setoid_rewrite <- in_rev.
+        destruct (rev t__R1) eqn:Heq. all:inv Hlast.
+        destruct t__R1. now inv Heq. inv H__R. eapply H'. reflexivity.  rewrite Hx;cbn;autorewrite with list;cbn. reflexivity.
+    Qed.
+
+    Lemma f_spec t b t':
+      f t = (b,t')
+      -> Rel [|t|] (b,[|t'|]).
+    Proof.
+      unfold f;cbn. destruct current eqn:Hcur.
+      2:{ intros [= <- <-];cbn;intros ? ? ?. destruct x;cbn;eexists;(split;[reflexivity| ]). all:intros ->;inv Hcur. }
+      destruct t as [ | | | t__L s' t__R];inversion Hcur. subst s';clear Hcur.
+      destruct isLeftBlank eqn:H__LB.
+      2:destruct isNilBlank eqn:H__NB.
+      2:{ intros [= <- <- ]. destruct s;inv H__NB. eexists (@niltape _),_,_;cbn. eauto 10. }
+      2:{ intros [= <- <- ]. intros ? x ?. destruct x;cbn;eexists;(split;[reflexivity | ]). all:destruct s;intros [= -> ->]. all:easy. }
+      destruct s;inv H__LB.
+      destruct t__R. 1:{ cbn. rewrite f'_equation. cbn. intros [= <- <-]. intros ? x ?. destruct x;cbn;eexists;(split;[reflexivity | ]). all:intros [= -> ->]. all:revert H0. all:length_not_eq. }
+      intros H';symmetry in H'. assert (H:=H'). revert H. intros H%(f'_spec (t__L':=[])).
+      2:now destruct marked;cbn;nia. 2:easy. 2:now constructor. destruct b;cbn  in H.
+      -destruct H as (x&t__R1&t__R2&->&Hx&->). all:destruct (rev (encode_tape x)) eqn:Hlast.
+       1:{ rewrite Hx in Hlast. exfalso;revert Hlast; length_not_eq. }
+       do 4 eexists.
+       +rewrite Hx;cbn. eauto.
+       +setoid_rewrite Hlast at 1. rewrite Hx in Hlast. cbn in Hlast.
+        apply (f_equal (hd e)) in Hlast. cbn in Hlast. rewrite hd_app in Hlast. 2: length_not_eq. subst s.
+        rewrite Hx. cbn. rewrite <- !tl_app. 2,3:length_not_eq. repeat (autorewrite with list;cbn). eauto 10.
+      -intros ? x ?. exists (hd NilBlank (encode_tape x)). split. now destruct x.
+       intros [= <- H1 H2]. destruct encode_tape eqn:Heqt. now inv H1. cbn in *. subst s.
+       destruct l. 1:{ destruct x;cbn in Heqt;try now inv Heqt. all:revert Heqt. all:length_not_eq. }
+       inv H2. eapply H. 2:exact Heqt. reflexivity.
+    Qed.
+
+
+  End checkEncodesTape.
+End CheckEncodesTape.
